internal/coq/coq.go
@@ -444,6 +444,15 @@ func (l StringLiteral) Coq() string {
 	return fmt.Sprintf(`#(str"%s")`, l.Value)
 }
 
+type nullLiteral struct{}
+
+func (l nullLiteral) Coq() string {
+	return "#null"
+}
+
+// Null represents a nil pointer in Go
+var Null = nullLiteral{}
+
 // BinOp is an enum for a Coq binary operator
 type BinOp int
 
